WIP

src/Specific/GF25519Reflective/Reified/Mul.v
@@ -1,6 +1,40 @@
-Require Import Crypto.Specific.GF25519Reflective.CommonBinOp.
+Require Export Crypto.Specific.GF25519Reflective.Common.
+Require Export Crypto.Reflection.Z.Interpretations.
+(*Require Import Crypto.Specific.GF25519Reflective.CommonBinOp.*)
 
 Definition rmulZ_sig : rexpr_binop_sig mul. Proof. reify_sig. Defined.
+Import Reflection.Syntax.
+Compute proj1_sig rmulZ_sig.
+Require Import Reflection.MapCastWithCastOp.
+Require Import Reflection.MapInterp.
+Goal True.
+  pose (proj1_sig rmulZ_sig) as e.
+  let T := type of e in
+  vm_compute in e;
+    change T in (type of e).
+  refine (let k := fun var
+                   => @map_interp_cast_with_cast_op
+                        base_type base_type interp_base_type Bounds.interp_base_type
+                        op op (@Bounds.interp_op)
+                        base_type_beq internal_base_type_dec_bl (fun _ => ZToInterp 0)
+                        (fun _ => Bounds.bounds_to_base_type)
+                        (fun _ _ v _ => cast_const v)
+                        (fun _ _ _ => Op (Cast _ _))
+                        (fun _ _ opc => match opc with Cast _ _ => true | _ => false end)
+                        (@Bounds.bound_op)
+                        var
+                        _ (e _)
+                        _ (MapInterp (@Bounds.of_interp) e _)
+                        (Application.interp_all_binders_for_to' ExprBinOp_bounds)
+          in _);
+    cbv beta in k.
+let T' := type of k in set (T := MapCast.new_type _ _ _ _) in k.
+vm_compute in T.
+subst T.
+Timeout 5 let T := type of k in
+vm_compute in k;
+change T in (type of k).
+
 Definition rmulW := Eval vm_compute in rword_of_Z rmulZ_sig.
 Lemma rmulW_correct_and_bounded_gen : correct_and_bounded_genT rmulW rmulZ_sig.
 Proof. rexpr_correct. Qed.
